theories/examples/switcher/switcher_preamble.v
@@ -31,7 +31,7 @@ Section Switcher_preamble.
   Definition export_table_entryN (C : CmptName) (a : Addr) : namespace :=
     (export_tableN C) .@ "entry" .@ a.
 
-  Program Definition execute_entry_point_register (wpcc wcgp : Word) :
+  Program Definition execute_entry_point_register (wpcc wcgp : Word) (nargs : nat) :
     (WORLD -n> (leibnizO CmptName) -n> (leibnizO Reg) -n> iPropO Σ) :=
     λne (W : WORLD) (C : CmptName) (reg : leibnizO Reg),
       (full_map reg ∧
@@ -43,18 +43,19 @@ Section Switcher_preamble.
            (⌜ ∃ csp_b csp_e, wstk = (WCap RWL Local csp_b csp_e csp_b) ⌝ ∧ interp W C wstk))
        )
        ∧
-       (∀ (r : RegName) (v : Word), (⌜r ∈ dom_arg_rmap⌝ → ⌜reg !! r = Some v⌝ → interp W C v)) ∧
+       (∀ (r : RegName) (v : Word), (⌜r ∈ dom_arg_rmap nargs⌝ → ⌜reg !! r = Some v⌝ → interp W C v)) ∧
+      (* TODO I think the zeroes are not necessary and we never rely in it *)
        (∀ (r : RegName),
-          (⌜r ∉ (dom_arg_rmap ∪ {[PC; cra; cgp; csp]})⌝ →  ⌜reg !! r = Some (WInt 0)⌝)))%I.
+          (⌜r ∉ (dom_arg_rmap nargs ∪ {[PC; cra; cgp; csp]})⌝ →  ⌜reg !! r = Some (WInt 0)⌝)))%I.
   Solve All Obligations with solve_proper.
 
   Program Definition execute_entry_point
-    (wpcc wcgp : Word) (regs : Reg) (cstk : CSTK) (Ws : list WORLD) (Cs : list CmptName)
+    (wpcc wcgp : Word) (regs : Reg) (cstk : CSTK) (Ws : list WORLD) (Cs : list CmptName) (nargs : nat)
     : (WORLD -n> (leibnizO CmptName) -n> iPropO Σ) :=
     (λne (W : WORLD) (C : CmptName),
       ( interp_continuation cstk Ws Cs
          ∗ ⌜frame_match Ws Cs cstk W C⌝
-         ∗ (execute_entry_point_register wpcc wcgp W C regs)
+         ∗ (execute_entry_point_register wpcc wcgp nargs W C regs)
          ∗ registers_pointsto regs
          ∗ region W C
          ∗ sts_full_world W C
@@ -71,20 +72,21 @@ Section Switcher_preamble.
        (∃ (g_tbl : Locality) (b_tbl e_tbl a_tbl : Addr)
           (bpcc epcc : Addr)
           (bcgp ecgp : Addr)
-          (nargs off : Z),
+          (nargs : nat) (off : Z),
            ⌜ w = WCap RO g_tbl b_tbl e_tbl a_tbl ⌝
            ∗ ⌜ (b_tbl <= a_tbl < e_tbl)%a ⌝
            ∗ ⌜ (b_tbl < (b_tbl ^+1))%a ⌝
            ∗ ⌜ ((b_tbl ^+1) < a_tbl)%a ⌝
-           ∗ ⌜ (0 <= nargs <= 7 )%Z ⌝
+           ∗ ⌜ (0 <= nargs <= 7 )%nat ⌝
            ∗ inv (export_table_PCCN C) ( b_tbl ↦ₐ WCap RX Global bpcc epcc bpcc)
            ∗ inv (export_table_CGPN C) ( (b_tbl ^+ 1)%a ↦ₐ WCap RW Global bcgp ecgp bcgp)
-           ∗ inv (export_table_entryN C a_tbl) ( a_tbl ↦ₐ WInt (encode_entry_point nargs off))
+           ∗ inv (export_table_entryN C a_tbl) ( a_tbl ↦ₐ WInt (encode_entry_point (Z.of_nat nargs) off))
+           ∗ w ↦□ₑ nargs
            ∗ □ ( ∀ regs cstk Ws Cs W', ⌜related_sts_priv_world W W'⌝ →
                    ▷ (execute_entry_point
                             (WCap RX Global bpcc epcc (bpcc ^+ off)%a)
                             (WCap RW Global bcgp ecgp bcgp)
-                            regs cstk Ws Cs W' C))
+                            regs cstk Ws Cs nargs W' C))
       )%I.
   Solve All Obligations with solve_proper.
 
@@ -93,7 +95,7 @@ Section Switcher_preamble.
 
   Lemma persistent_cond_ot_switcher :
     persistent_cond ot_switcher_prop.
-  Proof. intros [ [] ] ; cbn ; apply _. Qed.
+  Proof. intros [ [] ] ; cbn; apply _. Qed.
 
   Definition cframe_interp (frm : cframe) (a_tstk : Addr) : iProp Σ :=
     ∃ (wtstk4 : Word),
