theories/examples/switcher/switcher_spec.v
@@ -39,11 +39,12 @@ Section Switcher.
     (stk_mem : list Word)
     (arg_rmap rmap : Reg)
     (cstk : CSTK) (Ws : list WORLD) (Cs : list CmptName)
+    (nargs : nat)
     :
     let a_stk4 := (a_stk ^+ 4)%a in
     let wct1_caller := WSealed ot_switcher w_entry_point in
-    dom rmap = all_registers_s ∖ ({[ PC ; cgp ; cra ; csp ; ct1 ; cs0 ; cs1 ]} ∪ dom_arg_rmap) ->
-    is_arg_rmap arg_rmap ->
+    dom rmap = all_registers_s ∖ ({[ PC ; cgp ; cra ; csp ; ct1 ; cs0 ; cs1 ]} ∪ dom_arg_rmap nargs) ->
+    is_arg_rmap arg_rmap nargs ->
 
     (* Switcher Invariant *)
     na_inv logrel_nais Nswitcher switcher_inv
@@ -57,7 +58,7 @@ Section Switcher.
     (* Stack register *)
     ∗ csp ↦ᵣ WCap RWL Local b_stk e_stk a_stk
     (* Entry point of the target compartment *)
-    ∗ ct1 ↦ᵣ wct1_caller ∗ interp W C wct1_caller
+    ∗ ct1 ↦ᵣ wct1_caller ∗ interp W C wct1_caller ∗ wct1_caller ↦□ₑ nargs
     ∗ cs0 ↦ᵣ wcs0_caller
     ∗ cs1 ↦ᵣ wcs1_caller
     (* Argument registers, need to be safe-to-share *)
@@ -74,6 +75,7 @@ Section Switcher.
     ∗ ([∗ list] a ∈ (finz.seq_between a_stk e_stk), closing_revoked_resources W C a ∗ ⌜(std W) !! a = Some Revoked⌝)
     ∗ cstack_frag cstk
     ∗ interp_continuation cstk Ws Cs
+
 
     (* POST-CONDITION *)
     ∗ ▷ ( ∀ (W2 : WORLD) (rmap' : Reg),
