theories/ftlr/ftlr_base.v
@@ -8,6 +8,7 @@ Section fundamental.
   Context
     {Σ:gFunctors}
     {ceriseg:ceriseG Σ} {sealsg: sealStoreG Σ}
+    {entryg : entryGS Σ}
     {Cname : CmptNameG}
     {stsg : STSG Addr region_type Σ} {heapg : heapGS Σ}
     {cstackg : CSTACKG Σ}
