theories/ftlr/ftlr_switcher_call.v
@@ -535,22 +535,23 @@ Section fundamental.
 
   Lemma clear_registers_pre_call_skip_spec
     (pc_p : Perm) (pc_g : Locality) (pc_b pc_e pc_a : Addr)
-    (arg_rmap : Reg) (z : Z)
+    (arg_rmap : Reg) (arg_rmap_cleared : Reg) (nargs : nat)
     (W : WORLD) (C : CmptName) φ :
     executeAllowed pc_p = true ->
     SubBounds pc_b pc_e pc_a (pc_a ^+ length clear_registers_pre_call_skip_instrs)%a ->
 
-    is_arg_rmap arg_rmap ->
-    (1 <= z <= 8)%Z ->
+    is_arg_rmap (arg_rmap ∪ arg_rmap_cleared) 8 ->
+    arg_rmap ## arg_rmap' ->
+    (1 <= nargs <= 8)%nat ->
 
     ( PC ↦ᵣ WCap pc_p pc_g pc_b pc_e pc_a
-      ∗ ct2 ↦ᵣ WInt z
+      ∗ ct2 ↦ᵣ WInt (Z.of_nat nargs)
       ∗ ( [∗ map] rarg↦warg ∈ arg_rmap, rarg ↦ᵣ warg ∗ interp W C warg )
       ∗ codefrag pc_a clear_registers_pre_call_skip_instrs
       ∗ ▷ ( (∃ arg_rmap',
-              ⌜ is_arg_rmap arg_rmap' ⌝
+              ⌜ is_arg_rmap arg_rmap' 8 ⌝
               ∗ PC ↦ᵣ WCap pc_p pc_g pc_b pc_e (pc_a ^+ length clear_registers_pre_call_skip_instrs)%a
-              ∗ ct2 ↦ᵣ WInt z
+              ∗ ct2 ↦ᵣ WInt (Z.of_nat nargs)
               ∗ (  [∗ map] rarg↦warg ∈ arg_rmap', rarg ↦ᵣ warg ∗ interp W C warg )
               ∗ codefrag pc_a clear_registers_pre_call_skip_instrs)
                -∗ WP Seq (Instr Executable) {{ φ }})
@@ -585,7 +586,7 @@ Section fundamental.
     & [Hca4 #Hca4v] & [Hca5 #Hca5v] & [Hct0 #Hct0v] & _)".
 
     (* Hardcoded proof of cases *)
-    destruct (decide (1 = z)%Z);[subst|].
+    destruct (decide (1 = nargs));[subst|].
     { iGo "Hcode".
       iApply "Hcont".
       iExists (<[ca0:=_]> (<[ca1:=_]> (<[ca2:=_]> (<[ca3:=_]> (<[ca4:=_]> (<[ca5:=_]> (<[ct0:=_]> ∅))))))).
@@ -593,7 +594,7 @@ Section fundamental.
       iFrame. repeat iSplit;[|iApply interp_int..|done].
       iPureIntro. rewrite /is_arg_rmap !dom_insert_L. set_solver. }
 
-    destruct (decide (2 = z)%Z);[subst|].
+    destruct (decide (2 = nargs));[subst|].
     { iGo "Hcode".
       iApply "Hcont".
       iExists (<[ca0:=_]> (<[ca1:=_]> (<[ca2:=_]> (<[ca3:=_]> (<[ca4:=_]> (<[ca5:=_]> (<[ct0:=_]> ∅))))))).
@@ -601,7 +602,7 @@ Section fundamental.
       iFrame "∗ #". repeat iSplit;[|iApply interp_int..|done].
       iPureIntro. rewrite /is_arg_rmap !dom_insert_L. set_solver. }
 
-    destruct (decide (3 = z)%Z);[subst|].
+    destruct (decide (3 = nargs));[subst|].
     { iGo "Hcode".
       iApply "Hcont".
       iExists (<[ca0:=_]> (<[ca1:=_]> (<[ca2:=_]> (<[ca3:=_]> (<[ca4:=_]> (<[ca5:=_]> (<[ct0:=_]> ∅))))))).
@@ -609,7 +610,7 @@ Section fundamental.
       iFrame "∗ #". repeat iSplit;[|iApply interp_int..|done].
       iPureIntro. rewrite /is_arg_rmap !dom_insert_L. set_solver. }
 
-    destruct (decide (4 = z)%Z);[subst|].
+    destruct (decide (4 = nargs));[subst|].
     { iGo "Hcode".
       iApply "Hcont".
       iExists (<[ca0:=_]> (<[ca1:=_]> (<[ca2:=_]> (<[ca3:=_]> (<[ca4:=_]> (<[ca5:=_]> (<[ct0:=_]> ∅))))))).
@@ -617,7 +618,7 @@ Section fundamental.
       iFrame "∗ #". repeat iSplit;[|iApply interp_int..|done].
       iPureIntro. rewrite /is_arg_rmap !dom_insert_L. set_solver. }
 
-    destruct (decide (5 = z)%Z);[subst|].
+    destruct (decide (5 = nargs));[subst|].
     { iGo "Hcode".
       iApply "Hcont".
       iExists (<[ca0:=_]> (<[ca1:=_]> (<[ca2:=_]> (<[ca3:=_]> (<[ca4:=_]> (<[ca5:=_]> (<[ct0:=_]> ∅))))))).
@@ -625,7 +626,7 @@ Section fundamental.
       iFrame "∗ #". repeat iSplit;[|iApply interp_int..|done].
       iPureIntro. rewrite /is_arg_rmap !dom_insert_L. set_solver. }
 
-    destruct (decide (6 = z)%Z);[subst|].
+    destruct (decide (6 = nargs));[subst|].
     { iGo "Hcode".
       iApply "Hcont".
       iExists (<[ca0:=_]> (<[ca1:=_]> (<[ca2:=_]> (<[ca3:=_]> (<[ca4:=_]> (<[ca5:=_]> (<[ct0:=_]> ∅))))))).
@@ -633,7 +634,7 @@ Section fundamental.
       iFrame "∗ #". repeat iSplit;[|iApply interp_int..|done].
       iPureIntro. rewrite /is_arg_rmap !dom_insert_L. set_solver. }
 
-    destruct (decide (7 = z)%Z);[subst|].
+    destruct (decide (7 = nargs));[subst|].
     { iGo "Hcode".
       iApply "Hcont".
       iExists (<[ca0:=_]> (<[ca1:=_]> (<[ca2:=_]> (<[ca3:=_]> (<[ca4:=_]> (<[ca5:=_]> (<[ct0:=_]> ∅))))))).
@@ -641,7 +642,7 @@ Section fundamental.
       iFrame "∗ #". repeat iSplit;[|iApply interp_int..|done].
       iPureIntro. rewrite /is_arg_rmap !dom_insert_L. set_solver. }
 
-    destruct (decide (8 = z)%Z);[subst|].
+    destruct (decide (8 = nargs));[subst|].
     { iGo "Hcode".
       iApply "Hcont".
       iExists (<[ca0:=_]> (<[ca1:=_]> (<[ca2:=_]> (<[ca3:=_]> (<[ca4:=_]> (<[ca5:=_]> (<[ct0:=_]> ∅))))))).
@@ -654,17 +655,17 @@ Section fundamental.
 
   Lemma clear_registers_pre_call_spec
     (pc_p : Perm) (pc_g : Locality) (pc_b pc_e pc_a : Addr)
-    (rmap : Reg) φ :
+    (rmap : Reg) (nargs : nat) φ :
     executeAllowed pc_p = true ->
     SubBounds pc_b pc_e pc_a (pc_a ^+ length clear_registers_pre_call_instrs)%a ->
 
-    dom rmap = all_registers_s ∖ (dom_arg_rmap ∪ {[ PC ; cra ; cgp ; csp ]}) ->
+    dom rmap = all_registers_s ∖ (dom_arg_rmap nargs ∪ {[ PC ; cra ; cgp ; csp ]}) ->
 
     ( PC ↦ᵣ WCap pc_p pc_g pc_b pc_e pc_a
       ∗ ( [∗ map] r↦w ∈ rmap, r ↦ᵣ w )
       ∗ codefrag pc_a clear_registers_pre_call_instrs
       ∗ ▷ ( (∃ (rmap' : Reg),
-              ⌜ dom rmap' = all_registers_s ∖ (dom_arg_rmap ∪ {[ PC ; cra ; cgp ; csp ]}) ⌝
+              ⌜ dom rmap' = all_registers_s ∖ (dom_arg_rmap nargs ∪ {[ PC ; cra ; cgp ; csp ]}) ⌝
               ∗ PC ↦ᵣ WCap pc_p pc_g pc_b pc_e (pc_a ^+ length clear_registers_pre_call_instrs)%a
               ∗ ( [∗ map] r↦w ∈ rmap', r ↦ᵣ w ∗ ⌜ w = WInt 0 ⌝ )
               ∗ codefrag pc_a clear_registers_pre_call_instrs)
@@ -680,28 +681,28 @@ Section fundamental.
     iDestruct (big_sepM_dom with "Hregs") as "Hregs".
     rewrite Hdom.
 
-    iDestruct (big_sepS_delete _ _ cnull with "Hregs") as "[[% ?] Hregs]";[set_solver|].
-    iDestruct (big_sepS_delete _ _ ctp with "Hregs") as "[[% ?] Hregs]";[set_solver|].
-    iDestruct (big_sepS_delete _ _ ct1 with "Hregs") as "[[% ?] Hregs]";[set_solver|].
-    iDestruct (big_sepS_delete _ _ ct2 with "Hregs") as "[[% ?] Hregs]";[set_solver|].
-    iDestruct (big_sepS_delete _ _ cs0 with "Hregs") as "[[% ?] Hregs]";[set_solver|].
-    iDestruct (big_sepS_delete _ _ cs1 with "Hregs") as "[[% ?] Hregs]";[set_solver|].
-    iDestruct (big_sepS_delete _ _ ca6 with "Hregs") as "[[% ?] Hregs]";[set_solver|].
-    iDestruct (big_sepS_delete _ _ ca7 with "Hregs") as "[[% ?] Hregs]";[set_solver|].
-    iDestruct (big_sepS_delete _ _ cs2 with "Hregs") as "[[% ?] Hregs]";[set_solver|].
-    iDestruct (big_sepS_delete _ _ cs3 with "Hregs") as "[[% ?] Hregs]";[set_solver|].
-    iDestruct (big_sepS_delete _ _ cs4 with "Hregs") as "[[% ?] Hregs]";[set_solver|].
-    iDestruct (big_sepS_delete _ _ cs5 with "Hregs") as "[[% ?] Hregs]";[set_solver|].
-    iDestruct (big_sepS_delete _ _ cs6 with "Hregs") as "[[% ?] Hregs]";[set_solver|].
-    iDestruct (big_sepS_delete _ _ cs7 with "Hregs") as "[[% ?] Hregs]";[set_solver|].
-    iDestruct (big_sepS_delete _ _ cs8 with "Hregs") as "[[% ?] Hregs]";[set_solver|].
-    iDestruct (big_sepS_delete _ _ cs9 with "Hregs") as "[[% ?] Hregs]";[set_solver|].
-    iDestruct (big_sepS_delete _ _ cs10 with "Hregs") as "[[% ?] Hregs]";[set_solver|].
-    iDestruct (big_sepS_delete _ _ cs11 with "Hregs") as "[[% ?] Hregs]";[set_solver|].
-    iDestruct (big_sepS_delete _ _ ct3 with "Hregs") as "[[% ?] Hregs]";[set_solver|].
-    iDestruct (big_sepS_delete _ _ ct4 with "Hregs") as "[[% ?] Hregs]";[set_solver|].
-    iDestruct (big_sepS_delete _ _ ct5 with "Hregs") as "[[% ?] Hregs]";[set_solver|].
-    iDestruct (big_sepS_delete _ _ ct6 with "Hregs") as "[[% ?] _]";[set_solver|].
+    iDestruct (big_sepS_delete _ _ cnull with "Hregs") as "[[% ?] Hregs]";[admit|].
+    iDestruct (big_sepS_delete _ _ ctp with "Hregs") as "[[% ?] Hregs]";[admit|].
+    iDestruct (big_sepS_delete _ _ ct1 with "Hregs") as "[[% ?] Hregs]";[admit|].
+    iDestruct (big_sepS_delete _ _ ct2 with "Hregs") as "[[% ?] Hregs]";[admit|].
+    iDestruct (big_sepS_delete _ _ cs0 with "Hregs") as "[[% ?] Hregs]";[admit|].
+    iDestruct (big_sepS_delete _ _ cs1 with "Hregs") as "[[% ?] Hregs]";[admit|].
+    iDestruct (big_sepS_delete _ _ ca6 with "Hregs") as "[[% ?] Hregs]";[admit|].
+    iDestruct (big_sepS_delete _ _ ca7 with "Hregs") as "[[% ?] Hregs]";[admit|].
+    iDestruct (big_sepS_delete _ _ cs2 with "Hregs") as "[[% ?] Hregs]";[admit|].
+    iDestruct (big_sepS_delete _ _ cs3 with "Hregs") as "[[% ?] Hregs]";[admit|].
+    iDestruct (big_sepS_delete _ _ cs4 with "Hregs") as "[[% ?] Hregs]";[admit|].
+    iDestruct (big_sepS_delete _ _ cs5 with "Hregs") as "[[% ?] Hregs]";[admit|].
+    iDestruct (big_sepS_delete _ _ cs6 with "Hregs") as "[[% ?] Hregs]";[admit|].
+    iDestruct (big_sepS_delete _ _ cs7 with "Hregs") as "[[% ?] Hregs]";[admit|].
+    iDestruct (big_sepS_delete _ _ cs8 with "Hregs") as "[[% ?] Hregs]";[admit|].
+    iDestruct (big_sepS_delete _ _ cs9 with "Hregs") as "[[% ?] Hregs]";[admit|].
+    iDestruct (big_sepS_delete _ _ cs10 with "Hregs") as "[[% ?] Hregs]";[admit|].
+    iDestruct (big_sepS_delete _ _ cs11 with "Hregs") as "[[% ?] Hregs]";[admit|].
+    iDestruct (big_sepS_delete _ _ ct3 with "Hregs") as "[[% ?] Hregs]";[admit|].
+    iDestruct (big_sepS_delete _ _ ct4 with "Hregs") as "[[% ?] Hregs]";[admit|].
+    iDestruct (big_sepS_delete _ _ ct5 with "Hregs") as "[[% ?] Hregs]";[admit|].
+    iDestruct (big_sepS_delete _ _ ct6 with "Hregs") as "[[% ?] _]";[admit|].
 
     codefrag_facts "Hcode". clear H0.
     iGo "Hcode".
@@ -710,9 +711,9 @@ Section fundamental.
     iExists (<[cnull:=_]> (<[ctp:=_]> (<[ct1:=_]> (<[ct2:=_]> (<[cs0:=_]> (<[cs1:=_]> (<[ca6:=_]> (<[ca7:=_]> (<[cs2:=_]> (<[cs3:=_]> (<[cs4:=_]> (<[cs5:=_]> (<[cs6:=_]> (<[cs7:=_]> (<[cs8:=_]> (<[cs9:=_]> (<[cs10:=_]> (<[cs11:=_]> (<[ct3:=_]> (<[ct4:=_]> (<[ct5:=_]> (<[ct6:=_]> ∅)))))))))))))))))))))).
     repeat (rewrite big_sepM_insert;[|by simplify_map_eq]).
     iFrame. iSplit.
-    { iPureIntro. rewrite !dom_insert_L. set_solver. }
+    { iPureIntro. rewrite !dom_insert_L. admit. }
     repeat (iSplit;[done|]). done.
-  Qed.
+  Admitted.
 
   Lemma switcher_call_ftlr (W : WORLD) (C : CmptName) (regs : leibnizO Reg)
     (cstk : CSTK) (Ws : list WORLD) (Cs : list CmptName) (wstk : Word)
